Auto/Lib/HList.lean
@@ -1,3 +1,5 @@
+import Auto.Lib.HEqExtra
+
 namespace Auto
 
 inductive HList (β : α → Sort _) : List α → Sort _
@@ -37,14 +39,69 @@ def HList.map {β : α → Sort _} {γ : α → Sort _} (f : ∀ (a : α), β a 
   | .nil,      .nil       => .nil
   | .cons _ _, .cons x xs => .cons (f _ x) (map f xs)
 
+def HList.append : (xs : HList β as) → (ys : HList β bs) → HList β (as ++ bs)
+  | .nil,       ys => ys
+  | .cons x xs, ys => .cons x (append xs ys)
+
+theorem HList.append_assoc (xs : HList β as) (ys : HList β bs) (zs : HList β cs) :
+  HEq (append (append xs ys) zs) (append xs (append ys zs)) := by
+  induction xs
+  case nil => apply HEq.rfl
+  case cons a as x xs IH =>
+    dsimp [append];
+    apply congr_h_heq
+    case Hβ => rw [List.append_assoc]
+    case h₁ =>
+      apply congr_h_heq;
+      case Hβ => rw [List.append_assoc]
+      case h₁ =>
+        apply congr_hd_heq <;> try apply HEq.rfl;
+        rw [List.append_assoc]; apply HEq.rfl
+      case h₂ => apply HEq.rfl
+    case h₂ => exact IH
+
+theorem HList.getD_append_left (xs : HList β as) (ys : HList β bs) (h : i < as.length) :
+  HEq ((append xs ys).getD df i) (xs.getD df i) := by
+  induction xs generalizing i bs
+  case nil => contradiction
+  case cons a as x xs IH =>
+    dsimp [append]; cases i
+    case zero => apply HEq.rfl
+    case succ i =>
+      dsimp [getD]; apply IH; apply Nat.le_of_succ_le_succ h
+
+theorem HList.getD_append_right (xs : HList β as) (ys : HList β bs) (h : i ≥ as.length) :
+  HEq ((append xs ys).getD df i) (ys.getD df (i - as.length)) := by
+  induction xs generalizing i bs
+  case nil => apply HEq.rfl
+  case cons a as x xs IH =>
+    dsimp [append]; cases i
+    case zero => contradiction
+    case succ i =>
+      dsimp [getD]; rw [Nat.succ_sub_succ];
+      apply IH; apply Nat.le_of_succ_le_succ h
+
 def HList.reverseAux : {as : _} → (xs : HList β as) → (ys : HList β bs) → HList β (List.reverseAux as bs)
   | .nil,       .nil,       r => r
   | .cons _ as, .cons x xs, r => reverseAux (as:=as) xs (.cons x r)
 
 def HList.reverse (xs : HList β as) : HList β (List.reverse as) := HList.reverseAux xs .nil
 
-def HList.append : (xs : HList β as) → (ys : HList β bs) → HList β (as.append bs)
-  | .nil,       ys => ys
-  | .cons x xs, ys => .cons x (append xs ys)
+theorem HList.reverseAux_eq_append {xs : HList β as} {ys : HList β bs} :
+  HEq (reverseAux xs ys) (append (reverseAux xs .nil) ys) := by
+  induction xs generalizing bs ys
+  case nil => apply HEq.rfl
+  case cons a as x xs IH =>
+    dsimp [reverseAux]
+    apply HEq.trans (@IH (a :: bs) (.cons x ys))
+    apply HEq.trans (b:=append (append (reverseAux xs .nil) (cons x nil)) ys)
+    case h₁ =>
+      apply HEq.symm; apply HList.append_assoc
+    case h₂ =>
+      congr
+      case e_3.h =>
+        dsimp [List.reverseAux]; rw [List.reverseAux_eq_append _ [a]]
+      case e_5 =>
+        apply HEq.symm; apply IH
 
 end Auto
